Refactoring: Definitions stype -> proto, st -> prot

theories/proto/branching.v
@@ -9,21 +9,21 @@ Section DualBranch.
   Context `{PROP : bi}.
 
   Definition TSB (a : action)
-             (st1 st2 : stype val PROP) : stype val PROP :=
-    TSR' a (λ _, True)%I (λ v, if v : bool then st1 else st2).
+             (prot1 prot2 : proto val PROP) : proto val PROP :=
+    TSR' a (λ _, True)%I (λ v, if v : bool then prot1 else prot2).
 
-  Global Instance is_dual_tsb a1 a2 st1 st1' st2 st2' :
+  Global Instance is_dual_tsb a1 a2 proto1 proto1' proto2 proto2' :
     IsDualAction a1 a2 →
-    IsDualStype st1 st1' → IsDualStype st2 st2' →
-    IsDualStype (TSB a1 st1 st2) (TSB a2 st1' st2').
+    IsDualProto proto1 proto1' → IsDualProto proto2 proto2' →
+    IsDualProto (TSB a1 proto1 proto2) (TSB a2 proto1' proto2').
   Proof.
     rewrite /IsDualAction.
-    rewrite /IsDualStype.
+    rewrite /IsDualProto.
     intros Ha Hst1 Hst2.
     destruct a1.
     - simpl.
       simpl in Ha. rewrite -Ha.
-      rewrite -(stype_force_eq (dual_stype _)).
+      rewrite -(proto_force_eq (dual_proto _)).
       constructor.
       f_equiv.
       f_equiv.
@@ -31,7 +31,7 @@ Section DualBranch.
       by destruct b. apply is_dual_end.
     - simpl.
       simpl in Ha. rewrite -Ha.
-      rewrite -(stype_force_eq (dual_stype _)).
+      rewrite -(proto_force_eq (dual_proto _)).
       constructor.
       f_equiv.
       f_equiv.
@@ -42,8 +42,8 @@ Section DualBranch.
 End DualBranch.
 Global Typeclasses Opaque TSB.
 
-Infix "<+>" := (TSB Send) (at level 85) : stype_scope.
-Infix "<&>" := (TSB Receive) (at level 85) : stype_scope.
+Infix "<+>" := (TSB Send) (at level 85) : proto_scope.
+Infix "<&>" := (TSB Receive) (at level 85) : proto_scope.
 
 Section branching_specs.
   Context `{!heapG Σ} (N : namespace).
@@ -53,15 +53,15 @@ Section branching_specs.
     λ: "c" "s" "b",
       send "c" "s" "b".
 
-  Lemma select_st_spec st1 st2 γ c s (b : side) :
-    {{{ ⟦ c @ s : st1 <+> st2 ⟧{N,γ} }}}
+  Lemma select_st_spec proto1 proto2 γ c s (b : side) :
+    {{{ ⟦ c @ s : proto1 <+> proto2 ⟧{N,γ} }}}
       select c #s #b
-    {{{ RET #(); ⟦ c @ s : (if b then st1 else st2) ⟧{N,γ} }}}.
+    {{{ RET #(); ⟦ c @ s : (if b then proto1 else proto2) ⟧{N,γ} }}}.
   Proof.
-    iIntros (Φ) "Hst HΦ".
+    iIntros (Φ) "Hproto HΦ".
     wp_pures. wp_lam.
     wp_pures. rewrite /TSB.
-    wp_apply (send_st_spec N bool with "[$Hst //]");
+    wp_apply (send_st_spec N bool with "[$Hproto //]");
     iIntros "Hstl".
     iApply "HΦ".
     by destruct b.
@@ -73,17 +73,17 @@ Section branching_specs.
        then "b1"
        else "b2".
 
-  Lemma branch_st_spec st1 st2 γ c s (b1 b2 : val) :
-    {{{ ⟦ c @ s : st1 <&> st2 ⟧{N,γ} }}}
+  Lemma branch_st_spec proto1 proto2 γ c s (b1 b2 : val) :
+    {{{ ⟦ c @ s : proto1 <&> proto2 ⟧{N,γ} }}}
       branch c #s b1 b2
-    {{{ v, RET v; (⌜v = b1%V⌝ ∧ ⟦ c @ s : st1 ⟧{N,γ}) ∨
-                  (⌜v = b2%V⌝ ∧ ⟦ c @ s : st2 ⟧{N,γ})}}}.
+    {{{ v, RET v; (⌜v = b1%V⌝ ∧ ⟦ c @ s : proto1 ⟧{N,γ}) ∨
+                  (⌜v = b2%V⌝ ∧ ⟦ c @ s : proto2 ⟧{N,γ})}}}.
   Proof.
     iIntros (Φ').
-    iIntros "Hst HΦ'".
+    iIntros "Hproto HΦ'".
     wp_pures.
     wp_lam. rewrite /TSB. simpl.
-    wp_apply (recv_st_spec N bool with "[$Hst //]").
+    wp_apply (recv_st_spec N bool with "[$Hproto //]").
     iIntros (v) "[Hstl _]".
     destruct v.
     - wp_pures. iApply ("HΦ'"). eauto with iFrame.
