theories/proto/proto_def.v
@@ -14,273 +14,273 @@ Definition dual_action (a : action) : action :=
 Instance dual_action_involutive : Involutive (=) dual_action.
 Proof. by intros []. Qed.
 
-CoInductive stype (V A : Type) :=
+CoInductive proto (V A : Type) :=
   | TEnd
-  | TSR (a : action) (P : V → A) (st : V → stype V A).
+  | TSR (a : action) (P : V → A) (prot : V → proto V A).
 Arguments TEnd {_ _}.
 Arguments TSR {_ _} _ _ _.
 Instance: Params (@TSR) 3.
 
-Instance stype_inhabited V A : Inhabited (stype V A) := populate TEnd.
+Instance stype_inhabited V A : Inhabited (proto V A) := populate TEnd.
 
-CoFixpoint dual_stype {V A} (st : stype V A) : stype V A :=
-  match st with
+CoFixpoint dual_proto {V A} (prot : proto V A) : proto V A :=
+  match prot with
   | TEnd => TEnd
-  | TSR a P st => TSR (dual_action a) P (λ v, dual_stype (st v))
+  | TSR a P prot => TSR (dual_action a) P (λ v, dual_proto (prot v))
   end.
-Instance: Params (@dual_stype) 2.
+Instance: Params (@dual_proto) 2.
 
-Delimit Scope stype_scope with stype.
-Bind Scope stype_scope with stype.
+Delimit Scope proto_scope with proto.
+Bind Scope proto_scope with proto.
 
-Notation "<!> x @ P , st" :=
-  (TSR Send (λ x, P%I) (λ x, st%stype))
-  (at level 200, x pattern, st at level 200) : stype_scope.
-Notation "<?> x @ P , st" :=
-  (TSR Receive (λ x, P%I) (λ x, st%stype))
-  (at level 200, x pattern, st at level 200) : stype_scope.
-Notation "<!> x , st" := (<!> x @ True, st%stype)%stype
-  (at level 200, x pattern, st at level 200) : stype_scope.
-Notation "<?> x , st" := (<?> x @ True, st%stype)%stype
-  (at level 200, x pattern, st at level 200) : stype_scope.
-Notation "<!> @ P , st" := (<!> x @ P x, st x)%stype
-  (at level 200, st at level 200) : stype_scope.
-Notation "<?> @ P , st" := (<?> x @ P x, st x)%stype
-  (at level 200, st at level 200) : stype_scope.
+Notation "<!> x @ P , prot" :=
+  (TSR Send (λ x, P%I) (λ x, prot%proto))
+  (at level 200, x pattern, prot at level 200) : proto_scope.
+Notation "<?> x @ P , prot" :=
+  (TSR Receive (λ x, P%I) (λ x, prot%proto))
+  (at level 200, x pattern, prot at level 200) : proto_scope.
+Notation "<!> x , prot" := (<!> x @ True, prot%proto)%proto
+  (at level 200, x pattern, prot at level 200) : proto_scope.
+Notation "<?> x , prot" := (<?> x @ True, prot%proto)%proto
+  (at level 200, x pattern, prot at level 200) : proto_scope.
+Notation "<!> @ P , prot" := (<!> x @ P x, prot x)%proto
+  (at level 200, prot at level 200) : proto_scope.
+Notation "<?> @ P , prot" := (<?> x @ P x, prot x)%proto
+  (at level 200, prot at level 200) : proto_scope.
 
-Section stype_ofe.
+Section proto_ofe.
   Context {V : Type}.
   Context {A : ofeT}.
 
-  CoInductive stype_equiv : Equiv (stype V A) :=
+  CoInductive proto_equiv : Equiv (proto V A) :=
     | TEnd_equiv : TEnd ≡ TEnd
-    | TSR_equiv a P1 P2 st1 st2 :
+    | TSR_equiv a P1 P2 prot1 prot2 :
        pointwise_relation V (≡) P1 P2 →
-       pointwise_relation V (≡) st1 st2 →
-       TSR a P1 st1 ≡ TSR a P2 st2.
-  Existing Instance stype_equiv.
+       pointwise_relation V (≡) prot1 prot2 →
+       TSR a P1 prot1 ≡ TSR a P2 prot2.
+  Existing Instance proto_equiv.
 
-  CoInductive stype_dist : Dist (stype V A) :=
+  CoInductive proto_dist : Dist (proto V A) :=
     | TEnd_dist n : TEnd ≡{n}≡ TEnd
-    | TSR_dist_0 a P1 P2 st1 st2 :
+    | TSR_dist_0 a P1 P2 prot1 prot2 :
        pointwise_relation V (dist 0) P1 P2 →
-       TSR a P1 st1 ≡{0}≡ TSR a P2 st2
-    | TSR_dist_S n a P1 P2 st1 st2 :
+       TSR a P1 prot1 ≡{0}≡ TSR a P2 prot2
+    | TSR_dist_S n a P1 P2 prot1 prot2 :
        pointwise_relation V (dist (S n)) P1 P2 →
-       pointwise_relation V (dist n) st1 st2 →
-       TSR a P1 st1 ≡{S n}≡ TSR a P2 st2.
-  Existing Instance stype_dist.
+       pointwise_relation V (dist n) prot1 prot2 →
+       TSR a P1 prot1 ≡{S n}≡ TSR a P2 prot2.
+  Existing Instance proto_dist.
 
-  Lemma TSR_dist n a P1 P2 st1 st2 :
+  Lemma TSR_dist n a P1 P2 prot1 prot2 :
     pointwise_relation V (dist n) P1 P2 →
-    pointwise_relation V (dist_later n) st1 st2 →
-    TSR a P1 st1 ≡{n}≡ TSR a P2 st2.
+    pointwise_relation V (dist_later n) prot1 prot2 →
+    TSR a P1 prot1 ≡{n}≡ TSR a P2 prot2.
   Proof. destruct n; by constructor. Defined.
 
-  Definition stype_ofe_mixin : OfeMixin (stype V A).
+  Definition proto_ofe_mixin : OfeMixin (proto V A).
   Proof.
     split.
-    - intros st1 st2. split.
-      + revert st1 st2. cofix IH; destruct 1 as [|a P1 P2 st1' st2' HP]=> n.
+    - intros prot1 prot2. split.
+      + revert prot1 prot2. cofix IH; destruct 1 as [|a P1 P2 prot1' prot2' HP]=> n.
         { constructor. }
         destruct n as [|n].
         * constructor=> v. apply equiv_dist, HP.
         * constructor=> v. apply equiv_dist, HP. by apply IH.
-      + revert st1 st2. cofix IH=> -[|a1 P1 st1] -[|a2 P2 st2] Hst;
-          feed inversion (Hst O); subst; constructor=> v.
-        * apply equiv_dist=> n. feed inversion (Hst n); auto.
-        * apply IH=> n. feed inversion (Hst (S n)); auto.
+      + revert prot1 prot2. cofix IH=> -[|a1 P1 prot1] -[|a2 P2 prot2] Hprot;
+          feed inversion (Hprot O); subst; constructor=> v.
+        * apply equiv_dist=> n. feed inversion (Hprot n); auto.
+        * apply IH=> n. feed inversion (Hprot (S n)); auto.
     - intros n. split.
-      + revert n. cofix IH=> -[|n] [|a P st]; constructor=> v; auto.
+      + revert n. cofix IH=> -[|n] [|a P prot]; constructor=> v; auto.
       + revert n. cofix IH; destruct 1; constructor=> v; symmetry; auto.
       + revert n. cofix IH; destruct 1; inversion 1; constructor=> v; etrans; eauto.
     - cofix IH=> -[|n]; inversion 1; constructor=> v; try apply dist_S; auto.
   Qed.
-  Canonical Structure stypeC : ofeT := OfeT (stype V A) stype_ofe_mixin.
+  Canonical Structure protoC : ofeT := OfeT (proto V A) proto_ofe_mixin.
 
-  Definition stype_head (d : V -c> A) (st : stype V A) : V -c> A :=
-    match st with TEnd => d | TSR a P st => P end.
-  Definition stype_tail (v : V) (st : stypeC) : later stypeC :=
-    match st with TEnd => Next TEnd | TSR a P st => Next (st v) end.
-  Global Instance stype_head_ne d : NonExpansive (stype_head d).
+  Definition proto_head (d : V -c> A) (prot : proto V A) : V -c> A :=
+    match prot with TEnd => d | TSR a P prot => P end.
+  Definition proto_tail (v : V) (prot : protoC) : later protoC :=
+    match prot with TEnd => Next TEnd | TSR a P prot => Next (prot v) end.
+  Global Instance proto_head_ne d : NonExpansive (proto_head d).
   Proof. by destruct 1. Qed.
-  Global Instance stype_tail_ne v : NonExpansive (stype_tail v).
+  Global Instance proto_tail_ne v : NonExpansive (proto_tail v).
   Proof. destruct 1; naive_solver. Qed.
 
-  Definition stype_force (st : stype V A) : stype V A :=
-    match st with
+  Definition proto_force (prot : proto V A) : proto V A :=
+    match prot with
     | TEnd => TEnd
-    | TSR a P st => TSR a P st
+    | TSR a P prot => TSR a P prot
     end.
-  Lemma stype_force_eq st : stype_force st = st.
-  Proof. by destruct st. Defined.
+  Lemma proto_force_eq prot : proto_force prot = prot.
+  Proof. by destruct prot. Defined.
 
-  CoFixpoint stype_compl_go `{!Cofe A} (c : chain stypeC) : stypeC :=
+  CoFixpoint proto_compl_go `{!Cofe A} (c : chain protoC) : protoC :=
     match c O with
     | TEnd => TEnd
-    | TSR a P st => TSR a
-       (compl (chain_map (stype_head P) c) : V → A)
-       (λ v, stype_compl_go (later_chain (chain_map (stype_tail v) c)))
+    | TSR a P prot => TSR a
+       (compl (chain_map (proto_head P) c) : V → A)
+       (λ v, proto_compl_go (later_chain (chain_map (proto_tail v) c)))
     end.
 
-  Global Program Instance stype_cofe `{!Cofe A} : Cofe stypeC :=
-    {| compl c := stype_compl_go c |}.
+  Global Program Instance proto_cofe `{!Cofe A} : Cofe protoC :=
+    {| compl c := proto_compl_go c |}.
   Next Obligation.
     intros ? n c; rewrite /compl. revert c n. cofix IH=> c n.
-    rewrite -(stype_force_eq (stype_compl_go c)) /=.
-    destruct (c O) as [|a P st'] eqn:Hc0.
+    rewrite -(proto_force_eq (proto_compl_go c)) /=.
+    destruct (c O) as [|a P prot'] eqn:Hc0.
     - assert (c n ≡{0}≡ TEnd) as Hcn.
       { rewrite -Hc0 -(chain_cauchy c 0 n) //. lia. }
       by inversion Hcn.
-    - assert (c n ≡{0}≡ TSR a P st') as Hcn.
+    - assert (c n ≡{0}≡ TSR a P prot') as Hcn.
       { rewrite -Hc0 -(chain_cauchy c 0 n) //. lia. }
-      inversion Hcn as [|? P' ? st'' ? HP|]; subst.
+      inversion Hcn as [|? P' ? prot'' ? HP|]; subst.
       destruct n as [|n]; constructor.
-      + intros v. by rewrite (conv_compl 0 (chain_map (stype_head P) c) v) /= -H.
-      + intros v. by rewrite (conv_compl _ (chain_map (stype_head P) c) v) /= -H.
-      + intros v. assert (st'' v = later_car (stype_tail v (c (S n)))) as ->.
+      + intros v. by rewrite (conv_compl 0 (chain_map (proto_head P) c) v) /= -H.
+      + intros v. by rewrite (conv_compl _ (chain_map (proto_head P) c) v) /= -H.
+      + intros v. assert (prot'' v = later_car (proto_tail v (c (S n)))) as ->.
         { by rewrite -H /=. }
         apply IH.
   Qed.
 
-  Global Instance TSR_stype_contractive a n :
+  Global Instance TSR_proto_contractive a n :
     Proper (pointwise_relation _ (dist n) ==>
             pointwise_relation _ (dist_later n) ==> dist n) (TSR a).
   Proof. destruct n; by constructor. Qed.
-  Global Instance TSR_stype_ne a n :
+  Global Instance TSR_proto_ne a n :
     Proper (pointwise_relation _ (dist n) ==>
             pointwise_relation _ (dist n) ==> dist n) (TSR a).
   Proof.
-    intros P1 P2 HP st1 st2 Hst. apply TSR_stype_contractive=> //.
+    intros P1 P2 HP prot1 prot2 Hst. apply TSR_proto_contractive=> //.
     destruct n as [|n]=> // v /=. by apply dist_S.
   Qed.
-  Global Instance TSR_stype_proper a :
+  Global Instance TSR_proto_proper a :
     Proper (pointwise_relation _ (≡) ==>
             pointwise_relation _ (≡) ==> (≡)) (TSR a).
   Proof. by constructor. Qed.
 
-  Global Instance dual_stype_ne : NonExpansive dual_stype.
+  Global Instance dual_proto_ne : NonExpansive dual_proto.
   Proof.
-    cofix IH=> n st1 st2 Hst.
-    rewrite -(stype_force_eq (dual_stype st1)) -(stype_force_eq (dual_stype st2)).
+    cofix IH=> n prot1 prot2 Hst.
+    rewrite -(proto_force_eq (dual_proto prot1)) -(proto_force_eq (dual_proto prot2)).
     destruct Hst; constructor=> v; auto; by apply IH.
   Qed.
-  Global Instance dual_stype_proper : Proper ((≡) ==> (≡)) dual_stype.
+  Global Instance dual_proto_proper : Proper ((≡) ==> (≡)) dual_proto.
   Proof. apply (ne_proper _). Qed.
 
-  Global Instance dual_stype_involutive : Involutive (≡) dual_stype.
+  Global Instance dual_proto_involutive : Involutive (≡) dual_proto.
   Proof.
-    cofix IH=> st. rewrite -(stype_force_eq (dual_stype (dual_stype _))).
-    destruct st as [|a P st]; first done.
+    cofix IH=> prot. rewrite -(proto_force_eq (dual_proto (dual_proto _))).
+    destruct prot as [|a P prot]; first done.
     rewrite /= involutive. constructor=> v; auto.
   Qed.
 
-  Lemma stype_equivI {M} st1 st2 :
-    st1 ≡ st2 ⊣⊢@{uPredI M}
-        match st1, st2 with
+  Lemma proto_equivI {M} prot1 prot2 :
+    prot1 ≡ prot2 ⊣⊢@{uPredI M}
+        match prot1, prot2 with
         | TEnd, TEnd => True
-        | TSR a1 P1 st1, TSR a2 P2 st2 =>
-          ⌜ a1 = a2 ⌝ ∧ (∀ v, P1 v ≡ P2 v) ∧ ▷ (∀ v, st1 v ≡ st2 v)
+        | TSR a1 P1 prot1, TSR a2 P2 prot2 =>
+          ⌜ a1 = a2 ⌝ ∧ (∀ v, P1 v ≡ P2 v) ∧ ▷ (∀ v, prot1 v ≡ prot2 v)
         | _, _ => False
         end.
   Proof.
     uPred.unseal; constructor=> n x ?. split; first by destruct 1.
-    destruct st1, st2=> //=; [constructor|].
+    destruct prot1, prot2=> //=; [constructor|].
     by intros [[= ->] [??]]; destruct n; constructor.
   Qed.
 
-  Lemma stype_later_equiv M st a P2 st2 :
-    ▷ (st ≡ TSR a P2 st2) -∗
-    ◇ (∃ P1 st1, st ≡ TSR a P1 st1 ∗
+  Lemma proto_later_equiv M prot a P2 prot2 :
+    ▷ (prot ≡ TSR a P2 prot2) -∗
+    ◇ (∃ P1 prot1, prot ≡ TSR a P1 prot1 ∗
                  ▷ (∀ v, P1 v ≡ P2 v) ∗
-                 ▷ ▷ (∀ v, st1 v ≡ st2 v) : uPred M).
+                 ▷ ▷ (∀ v, prot1 v ≡ prot2 v) : uPred M).
   Proof.
-    iIntros "Heq". destruct st as [|a' P1 st1].
-    - iDestruct (stype_equivI with "Heq") as ">[]".
-    - iDestruct (stype_equivI with "Heq") as "(>-> & HPeq & Hsteq)".
-      iExists P1, st1. auto.
+    iIntros "Heq". destruct prot as [|a' P1 prot1].
+    - iDestruct (proto_equivI with "Heq") as ">[]".
+    - iDestruct (proto_equivI with "Heq") as "(>-> & HPeq & Hsteq)".
+      iExists P1, prot1. auto.
   Qed.
 
-  Lemma dual_stype_flip {M} st1 st2 :
-    dual_stype st1 ≡ st2 ⊣⊢@{uPredI M} st1 ≡ dual_stype st2.
+  Lemma dual_proto_flip {M} prot1 prot2 :
+    dual_proto prot1 ≡ prot2 ⊣⊢@{uPredI M} prot1 ≡ dual_proto prot2.
   Proof.
     iSplit.
-    - iIntros "Heq". iRewrite -"Heq". by rewrite dual_stype_involutive.
-    - iIntros "Heq". iRewrite "Heq". by rewrite dual_stype_involutive.
+    - iIntros "Heq". iRewrite -"Heq". by rewrite dual_proto_involutive.
+    - iIntros "Heq". iRewrite "Heq". by rewrite dual_proto_involutive.
   Qed.
-End stype_ofe.
+End proto_ofe.
 
-Arguments stypeC : clear implicits.
+Arguments protoC : clear implicits.
 
-CoFixpoint stype_map {V A B} (f : A → B) (st : stype V A) : stype V B :=
-  match st with
+CoFixpoint proto_map {V A B} (f : A → B) (prot : proto V A) : proto V B :=
+  match prot with
   | TEnd => TEnd
-  | TSR a P st => TSR a (λ v, f (P v)) (λ v, stype_map f (st v))
+  | TSR a P prot => TSR a (λ v, f (P v)) (λ v, proto_map f (prot v))
   end.
-Lemma stype_map_ext_ne {V A} {B : ofeT} (f g : A → B) (st : stype V A) n :
-  (∀ x, f x ≡{n}≡ g x) → stype_map f st ≡{n}≡ stype_map g st.
+Lemma proto_map_ext_ne {V A} {B : ofeT} (f g : A → B) (prot : proto V A) n :
+  (∀ x, f x ≡{n}≡ g x) → proto_map f prot ≡{n}≡ proto_map g prot.
 Proof.
-  revert n st. cofix IH=> n st Hf.
-  rewrite -(stype_force_eq (stype_map f st)) -(stype_force_eq (stype_map g st)).
-  destruct st as [|a P st], n as [|n]; constructor=> v //. apply IH; auto using dist_S.
+  revert n prot. cofix IH=> n prot Hf.
+  rewrite -(proto_force_eq (proto_map f prot)) -(proto_force_eq (proto_map g prot)).
+  destruct prot as [|a P prot], n as [|n]; constructor=> v //. apply IH; auto using dist_S.
 Qed.
-Lemma stype_map_ext {V A} {B : ofeT} (f g : A → B) (st : stype V A) :
-  (∀ x, f x ≡ g x) → stype_map f st ≡ stype_map g st.
+Lemma proto_map_ext {V A} {B : ofeT} (f g : A → B) (prot : proto V A) :
+  (∀ x, f x ≡ g x) → proto_map f prot ≡ proto_map g prot.
 Proof.
-  intros Hf. apply equiv_dist=> n. apply stype_map_ext_ne=> v.
+  intros Hf. apply equiv_dist=> n. apply proto_map_ext_ne=> v.
   apply equiv_dist, Hf.
 Qed.
-Instance stype_map_ne {V : Type} {A B : ofeT} (f : A → B) n :
+Instance proto_map_ne {V : Type} {A B : ofeT} (f : A → B) n :
   (∀ n, Proper (dist n ==> dist n) f) →
-  Proper (dist n ==> dist n) (@stype_map V _ _ f).
+  Proper (dist n ==> dist n) (@proto_map V _ _ f).
 Proof.
-  intros Hf. revert n. cofix IH=> n st1 st2 Hst.
-  rewrite -(stype_force_eq (stype_map _ st1)) -(stype_force_eq (stype_map _ st2)).
+  intros Hf. revert n. cofix IH=> n prot1 prot2 Hst.
+  rewrite -(proto_force_eq (proto_map _ prot1)) -(proto_force_eq (proto_map _ prot2)).
   destruct Hst; constructor=> v; apply Hf || apply IH; auto.
 Qed.
-Lemma stype_fmap_id {V : Type} {A : ofeT} (st : stype V A) :
-  stype_map id st ≡ st.
+Lemma proto_fmap_id {V : Type} {A : ofeT} (prot : proto V A) :
+  proto_map id prot ≡ prot.
 Proof.
-  revert st. cofix IH=> st. rewrite -(stype_force_eq (stype_map _ _)).
-  destruct st; constructor=> v; auto.
+  revert prot. cofix IH=> prot. rewrite -(proto_force_eq (proto_map _ _)).
+  destruct prot; constructor=> v; auto.
 Qed.
-Lemma stype_fmap_compose {V : Type} {A B C : ofeT} (f : A → B) (g : B → C) st :
-  stype_map (g ∘ f) st ≡ stype_map g (@stype_map V _ _ f st).
+Lemma proto_fmap_compose {V : Type} {A B C : ofeT} (f : A → B) (g : B → C) prot :
+  proto_map (g ∘ f) prot ≡ proto_map g (@proto_map V _ _ f prot).
 Proof.
-  revert st. cofix IH=> st.
-  rewrite -(stype_force_eq (stype_map _ _)) -(stype_force_eq (stype_map g _)).
-  destruct st; constructor=> v; auto.
+  revert prot. cofix IH=> prot.
+  rewrite -(proto_force_eq (proto_map _ _)) -(proto_force_eq (proto_map g _)).
+  destruct prot; constructor=> v; auto.
 Qed.
 
-Definition stypeC_map {V A B} (f : A -n> B) : stypeC V A -n> stypeC V B :=
-  CofeMor (stype_map f : stypeC V A → stypeC V B).
-Instance stypeC_map_ne {V} A B : NonExpansive (@stypeC_map V A B).
-Proof. intros n f g ? st. by apply stype_map_ext_ne. Qed.
+Definition protoC_map {V A B} (f : A -n> B) : protoC V A -n> protoC V B :=
+  CofeMor (proto_map f : protoC V A → protoC V B).
+Instance protoC_map_ne {V} A B : NonExpansive (@protoC_map V A B).
+Proof. intros n f g ? prot. by apply proto_map_ext_ne. Qed.
 
-Program Definition stypeCF {V} (F : cFunctor) : cFunctor := {|
-  cFunctor_car A _ B _ := stypeC V (cFunctor_car F A _ B _);
-  cFunctor_map A1 _ A2 _ B1 _ B2 _ fg := stypeC_map (cFunctor_map F fg)
+Program Definition protoCF {V} (F : cFunctor) : cFunctor := {|
+  cFunctor_car A _ B _ := protoC V (cFunctor_car F A _ B _);
+  cFunctor_map A1 _ A2 _ B1 _ B2 _ fg := protoC_map (cFunctor_map F fg)
 |}.
 Next Obligation. done. Qed.
 Next Obligation.
   by intros V F A1 ? A2 ? B1 ? B2 ? n f g Hfg;
-  apply stypeC_map_ne, cFunctor_ne.
+  apply protoC_map_ne, cFunctor_ne.
 Qed.
 Next Obligation.
-  intros V F A ? B ? x. rewrite /= -{2}(stype_fmap_id x).
-  apply stype_map_ext=>y. apply cFunctor_id.
+  intros V F A ? B ? x. rewrite /= -{2}(proto_fmap_id x).
+  apply proto_map_ext=>y. apply cFunctor_id.
 Qed.
 Next Obligation.
   intros V F A1 ? A2 ? A3 ? B1 ? B2 ? B3 ? f g f' g' x.
-  rewrite /= -stype_fmap_compose.
-  apply stype_map_ext=>y; apply cFunctor_compose.
+  rewrite /= -proto_fmap_compose.
+  apply proto_map_ext=>y; apply cFunctor_compose.
 Qed.
 
-Instance stypeCF_contractive {V} F :
-  cFunctorContractive F → cFunctorContractive (@stypeCF V F).
+Instance protoCF_contractive {V} F :
+  cFunctorContractive F → cFunctorContractive (@protoCF V F).
 Proof.
   by intros ? A1 ? A2 ? B1 ? B2 ? n f g Hfg;
-  apply stypeC_map_ne, cFunctor_contractive.
+  apply protoC_map_ne, cFunctor_contractive.
 Qed.
 
 Class IsDualAction (a1 a2 : action) :=
@@ -292,26 +292,26 @@ Proof. done. Qed.
 Instance is_dual_action_Receive : IsDualAction Receive Send.
 Proof. done. Qed.
 
-Section DualStype.
+Section DualProto.
   Context {V : Type} {A : ofeT}.
 
-  Class IsDualStype (st1 st2 : stype V A) :=
-  is_dual_stype : dual_stype st1 ≡ st2.
+  Class IsDualProto (prot1 prot2 : proto V A) :=
+  is_dual_proto : dual_proto prot1 ≡ prot2.
 
-  Global Instance is_dual_default (st : stype V A) :
-    IsDualStype st (dual_stype st) | 100.
-  Proof. by rewrite /IsDualStype. Qed.
+  Global Instance is_dual_default (prot : proto V A) :
+    IsDualProto prot (dual_proto prot) | 100.
+  Proof. by rewrite /IsDualProto. Qed.
 
-  Global Instance is_dual_end : IsDualStype (TEnd : stype V A) TEnd.
-  Proof. by rewrite /IsDualStype -(stype_force_eq (dual_stype _)). Qed.
+  Global Instance is_dual_end : IsDualProto (TEnd : proto V A) TEnd.
+  Proof. by rewrite /IsDualProto -(proto_force_eq (dual_proto _)). Qed.
 
-  Global Instance is_dual_tsr a1 a2 P (st1 st2 : V → stype V A) :
+  Global Instance is_dual_tsr a1 a2 P (prot1 prot2 : V → proto V A) :
     IsDualAction a1 a2 →
-    (∀ x, IsDualStype (st1 x) (st2 x)) →
-    IsDualStype (TSR a1 P st1) (TSR a2 P st2).
+    (∀ x, IsDualProto (prot1 x) (prot2 x)) →
+    IsDualProto (TSR a1 P prot1) (TSR a2 P prot2).
   Proof.
-    rewrite /IsDualAction /IsDualStype. intros <- Hst.
-    rewrite /IsDualStype -(stype_force_eq (dual_stype _)) /=.
+    rewrite /IsDualAction /IsDualProto. intros <- Hst.
+    rewrite /IsDualProto -(proto_force_eq (dual_proto _)) /=.
     by constructor=> v.
   Qed.
-End DualStype.
+End DualProto.
